Optimizations/Canonicalizations/TacticSolving.thy
@@ -1,0 +1,121 @@
+theory TacticSolving
+  imports Common
+begin
+
+fun size :: "IRExpr \<Rightarrow> nat" where
+  "size (UnaryExpr op e) = (size e) * 2" |
+  "size (BinaryExpr BinAdd x y) = (size x) + ((size y) * 2)" |
+  "size (BinaryExpr op x y) = (size x) + (size y)" |
+  "size (ConditionalExpr cond t f) = (size cond) + (size t) + (size f) + 2" |
+  "size (ConstantExpr c) = 1" |
+  "size (ParameterExpr ind s) = 2" |
+  "size (LeafExpr nid s) = 2" |
+  "size (ConstantVar c) = 2" |
+  "size (VariableExpr x s) = 2"
+
+lemma size_pos[simp]: "0 < size y"
+  apply (induction y; auto?)
+  subgoal premises prems for op a b
+    using prems by (induction op; auto)
+  done
+
+phase TacticSolving
+  terminating size
+begin
+
+subsection \<open>AddNode\<close>
+(*lemma val_add_left_negate_to_sub:
+  "val[-x + y] \<approx> val[y - x]"
+  apply simp by (cases x; cases y; auto)
+
+lemma exp_add_left_negate_to_sub:
+  "exp[-x + y] \<ge> exp[y - x]"
+  using val_add_left_negate_to_sub by auto*)
+
+lemma value_approx_implies_refinement:
+  assumes "lhs \<approx> rhs"
+  assumes "\<forall>m p v. ([m, p] \<turnstile> elhs \<mapsto> v) \<longrightarrow> v = lhs"
+  assumes "\<forall>m p v. ([m, p] \<turnstile> erhs \<mapsto> v) \<longrightarrow> v = rhs"
+  assumes "\<forall>m p v1 v2. ([m, p] \<turnstile> elhs \<mapsto> v1) \<longrightarrow> ([m, p] \<turnstile> erhs \<mapsto> v2)"
+  shows "elhs \<ge> erhs"
+  using assms unfolding le_expr_def well_formed_equal_def
+  using evalDet evaltree_not_undef
+  by metis
+
+method explore_cases for x y :: Value =
+  (cases x; cases y; auto)
+
+method explore_cases_bin for x :: IRExpr =
+  (cases x; auto)
+
+method obtain_approx_eq for lhs rhs x y :: Value =
+  (rule meta_mp[where P="lhs \<approx> rhs"], defer_tac, explore_cases x y)
+
+method obtain_eval for exp::IRExpr and val::Value =
+  (rule meta_mp[where P="\<And>m p v. ([m, p] \<turnstile> exp \<mapsto> v) \<Longrightarrow> v = val"], defer_tac)
+
+method solve for lhs rhs x y :: Value =
+  (match conclusion in "size _ < size _" \<Rightarrow> \<open>simp\<close>)?,
+  (match conclusion in "(elhs::IRExpr) \<ge> (erhs::IRExpr)" for elhs erhs \<Rightarrow> \<open>
+    (obtain_approx_eq lhs rhs x y)?\<close>)
+
+
+print_methods
+(*
+    (simp del: well_formed_equal_def le_expr_def)?;
+    ((rule allI)+)?\<close>)*)
+thm BinaryExprE
+optimization opt_add_left_negate_to_sub:
+  "-x + y \<longmapsto> y - x"
+  (*defer apply simp apply (rule allI)+ apply (rule impI)
+   apply (subgoal_tac "\<forall>x1. [m, p] \<turnstile> exp[-x + y] \<mapsto> x1") defer
+  *)
+   apply (solve "val[-x1 + y1]" "val[y1 - x1]" x1 y1)
+  apply simp apply auto using evaltree_not_undef sorry
+(*
+  apply (obtain_eval "exp[-x + y]" "val[-x1 + y1]")
+  
+
+  apply (rule BinaryExprE)
+  apply (rule allI)+ sorry
+  apply (auto simp: unfold_evaltree) sorry*)
+  (*
+   defer apply (test "val[-x1 + y1]" "val[y1 - x1]" x1 y1)
+   apply (rule meta_mp[where P="val[-x1 + y1] \<approx> val[y1 - x1]"])
+    prefer 2 apply (cases x1; cases y1; auto)
+   apply (subgoal_tac "val[-x1 + y1] \<approx> val[y1 - x1]")
+    apply (cases x1; cases y1; auto)
+  using exp_add_left_negate_to_sub apply simp
+  unfolding size.simps by simp*)
+
+subsection \<open>NegateNode\<close>
+
+lemma val_distribute_sub: 
+ "val[-(x-y)] \<approx> val[y-x]" 
+  by (cases x; cases y; auto) 
+
+optimization distribute_sub: "-(x-y) \<longmapsto> (y-x)" 
+  apply simp
+  using val_distribute_sub apply simp
+  using unfold_binary unfold_unary by auto
+
+lemma val_xor_self_is_false:
+  assumes "is_IntVal32 x"
+  shows "val[x \<oplus> x] \<approx> val[false]"
+  apply simp using assms by (cases x; auto)
+
+definition wf_stamp :: "IRExpr \<Rightarrow> bool" where
+  "wf_stamp e = (\<forall>m p v. ([m, p] \<turnstile> e \<mapsto> v) \<longrightarrow> valid_value v (stamp_expr e))"
+
+
+lemma exp_xor_self_is_false: 
+  assumes "stamp_expr x = IntegerStamp 32 l h"
+  assumes "wf_stamp x"
+  shows "exp[x \<oplus> x] >= exp[false]"
+  unfolding le_expr_def using assms unfolding wf_stamp_def
+  using val_xor_self_is_false evaltree_not_undef
+  by (metis BinaryExprE Value.disc(2) bin_eval.simps(6) evalDet unfold_const32 valid_int32 well_formed_equal_defn)
+
+end
+
+end
